src/OpSpec.v
@@ -2,30 +2,37 @@ Require Import List BaseTypes Memx Predx.
 Require Import CommonAutomation SepAuto Layer1 ProgAuto HoareL1.
 Open Scope pred_scope.
 
+Lemma star_split:
+    forall (AT : Type) (AEQ : EqDec AT) (V : Type)
+      (p q : @pred AT AEQ V) (m : @mem AT AEQ V),
+      (p * q)%pred m ->
+      (exists m1 m2, mem_disjoint m1 m2 /\ p m1 /\ q m2 /\ mem_union m1 m2 = m)%type.
+  Proof.
+    intros; unfold sep_star in *; rewrite sep_star_is in *;
+      destruct H; cleanup; eauto.
+    do 2 eexists; intuition eauto.
+  Qed.
+
 Theorem read_okay:
-  forall a v t ox,
+  forall a v,
     << o >>
-     (a |-> v * [[ o = t::ox ]])
+     (a |-> v)
      (Read a)
     << o', r >>
      (a |-> v *
-      [[ o' = ox ]] *
       [[r = fst v]])
-     (a |-> v *
-     [[ o' = ox ]]).
+     (a |-> v).
 Proof.
-  intros.
-  unfold hoare_triple; intros.
-  destruct_lift H; subst.
+  unfold hoare_triple; intros. 
   eapply ptsto_valid' in H as Hx;
-    cleanup; eauto.
-  destruct t; do 2 eexists;
+  cleanup; eauto.
+  destruct o.
+  destruct t; do 2 eexists.
     intuition eauto.
   econstructor; intuition eauto.
   inversion H0.
-  right; eexists; split; eauto.
-  pred_apply; cancel.
-  
+
+  intuition.
   econstructor; intuition eauto.
   unfold Disk.read in *; cleanup; eauto.
   left; do 2 eexists; split; eauto.
@@ -33,60 +40,50 @@ Proof.
 Qed.
 
 Theorem write_okay:
-  forall a v v' t ox,
+  forall a v v',
     << o >>
-     (a |-> v * [[ o = t::ox ]])
+     (a |-> v)
      (Write a v')
     << o', r >>
-     (a |-> (v', (fst v::snd v)) *
-      [[ o' = ox ]])
-     (a |-> v *
-      [[ o' = ox ]]).
+     (a |-> (v', (fst v::snd v)))
+     (a |-> v).
 Proof.
   intros.
   unfold hoare_triple; intros.
-  destruct_lift H; subst.
   eapply ptsto_valid' in H as Hx;
     cleanup; eauto.
   
-  destruct t; do 2 eexists;
+  destruct o, t; do 2 eexists.
     intuition eauto.
   econstructor; intuition eauto.
   inversion H0.
-  right; eexists; split; eauto.
-  pred_apply; cancel.
 
+  split.
   econstructor; intuition eauto.
   unfold Disk.read in *; cleanup; eauto.
   left; do 2 eexists; split; eauto.
   unfold Disk.write; cleanup.
   unfold Disk.upd_disk.
-  eapply ptsto_upd' in H.
-  pred_apply' H; cancel; eauto.
+  eapply ptsto_upd'; eauto.
 Qed.
 
 Theorem ret_okay:
-  forall T (v: T) t ox,
+  forall T (v: T),
     << o >>
-     (emp * [[ o = t::ox ]])
+     (emp)
      (Ret v)
     << o', r >>
     (emp *
-     [[r = v]] *
-     [[ o' = ox ]])
-    (emp *
-     [[o' = ox]]).
+     [[r = v]])
+    (emp).
 Proof.
   intros.
   unfold hoare_triple; intros.
-  destruct_lift H; subst.
-  destruct t; do 2 eexists;
+  
+  destruct o, t; do 2 eexists;
     intuition eauto.  
   econstructor; intuition eauto.
   inversion H0.
-  simpl in *; cleanup; right; eexists; intuition eauto.
-  pred_apply; cancel.
-
   left; do 2 eexists; split; eauto.
   pred_apply; cancel; eauto.
 Qed.
